wip

ref-jasmin/params/auto/gen_params.c
@@ -59,7 +59,7 @@ static void cleanup_file_path(char *filepath) {
     }
 }
 
-static void print_xmss_params(const char *_impl, xmss_params *p, uint32_t oid) {
+static void print_xmss_params(const char *_impl, const xmss_params *p, uint32_t oid) {
     if (!p || !_impl) {
         return;
     }
@@ -111,6 +111,8 @@ static void print_xmss_params(const char *_impl, xmss_params *p, uint32_t oid) {
     print_param(f, "XMSS_PK_BYTES", p->pk_bytes);
     print_param(f, "XMSS_SK_BYTES", p->sk_bytes);
     // print_param(f, "XMSS_BDS_K", p->bds_k);
+
+    print_param(f, "XMSS_REDUCED_SIG_BYTES", p->wots_sig_bytes + (p->tree_height * p->n));
 
     fclose(f);
 }
