proof/correctness/SignProof.ec
@@ -3,13 +3,13 @@ pragma Goals : printall.
 require import AllCore List RealExp IntDiv Distr DList IntDiv.
 from Jasmin require import JModel JArray.
 
-require import Params Types Hash XMSS_MT_PRF.
+require import Params Types Hash XMSS_MT_PRF XMSS_MT_Types XMSS_MT_Params.
 require import XMSS_IMPL Parameters.
 
 require import Repr2. 
 require import Utils2.
 
-require import Array3 Array8 Array32 Array64 Array68 Array96 Array131 Array352 Array2144.
+require import Array3 Array8 Array32 Array64 Array68 Array96 Array131 Array352 Array2144 Array4963.
 require import WArray32 WArray96 WArray131.
 
 require import Correctness_Address Correctness_Bytes Correctness_Mem Correctness_Hash.
@@ -20,18 +20,6 @@ require import BitEncoding.
 
 require import StdBigop. 
 (*---*) import Bigint.
-
-(*
-
-arg{1}.`1 => sk
-arg{1}.`2 => sm_ptr (* pointer to signed message *)
-arg{1}.`3 => smlen  (* length of signed message *)
-arg{1}.`4 => m_ptr  (* pointer to message *)
-arg{1}.`5 => mlen   (* length of the message *)
-
-arg{2}.`1 => sk
-arg{2}.`2 => msg
-*)
 
 lemma sign_invalid_idx :
     hoare [
@@ -71,22 +59,30 @@ seq 4 : (2 ^ XMSS_FULL_HEIGHT < to_uint idx).
 seq 1 : (#pre /\ #post /\ exit_0 = W8.one); last by rcondf 1; auto.
  
 rcondt 1; auto => /> ?; rewrite /XMSS_FULL_HEIGHT /= => ?; last by smt(@W64 pow2_64).
-rewrite /(`<<`) ifT // ultE /= /#.
+by rewrite /(`<<`) ifT // ultE /= /#.
+
 qed.
 
 
-op load_message (mem : global_mem_t) (ptr : W64.t) (mlen : W64.t) =
-  mkseq (fun (i : int) => mem.[to_uint ptr + i]) (to_uint mlen).
+op load_message (mem : global_mem_t) (ptr : W64.t) (len : W64.t) =
+  mkseq (fun (i : int) => mem.[to_uint ptr + i]) (to_uint len).
 
 
-lemma sign_correct (mem : global_mem_t) (_sk : xmss_sk, _sm_ptr _smlen_ptr _m_ptr _mlen : W64.t) :
+(*
+proc __xmssmt_core_sign (sk:W8.t Array131.t, sm_ptr:W64.t, smlen_ptr:W64.t,
+                           m_ptr:W64.t, mlen:W64.t) : W8.t Array131.t * W64.t 
+
+proc sign(sk : xmss_sk, m : msg_t) : sig_t * xmss_sk
+*)
+
+lemma sign_correct (_sk : xmss_sk, _sm_ptr _smlen_ptr _m_ptr _mlen : W64.t) :
     n = XMSS_N /\ 
+    d = XMSS_D /\
+    h = XMSS_FULL_HEIGHT /\
     prf_padding_val = XMSS_HASH_PADDING_PRF /\ 
     padding_len = XMSS_PADDING_LEN =>
     equiv [
       M(Syscall).__xmssmt_core_sign ~ XMSS_MT_PRF.sign :
-      Glob.mem{1} = mem /\
-      Glob.mem{2} = mem /\
 
       arg{1}.`1 = DecodeSkNoOID _sk /\
       arg{1}.`2 = _sm_ptr /\
@@ -95,15 +91,19 @@ lemma sign_correct (mem : global_mem_t) (_sk : xmss_sk, _sm_ptr _smlen_ptr _m_pt
       arg{1}.`5 = _mlen  /\
 
       arg{2}.`1 =_sk /\
-      arg{2}.`2 = load_message mem _m_ptr _mlen /\
+      arg{2}.`2 = load_message Glob.mem{1} _m_ptr _mlen /\
 
       valid_ptr_i arg{1}.`5 2500 /\
-      0 <= to_uint sk{2}.`idx < 2^XMSS_FULL_HEIGHT - 1 (* ensures that the maximum number of signatures was not yet reached *)
+      to_uint _sm_ptr + XMSS_SIG_BYTES <= W64.max_uint /\
+      0 <= to_uint _mlen <= W64.max_uint - XMSS_SIG_BYTES /\
+      0 <= to_uint sk{2}.`idx <= 2^XMSS_FULL_HEIGHT - 1 (* ensures that the maximum number of signatures was not yet reached *)
       ==>
-      res{2}.`2 = DecodeSkNoOID res{2}.`1
+      res{1}.`1 = DecodeSkNoOID res{2}.`2 /\
+      res{1}.`2 = W64.zero /\
+      res{2}.`1 = EncodeSignature  (load_message Glob.mem{1} _sm_ptr (W64.of_int XMSS_SIG_BYTES))
     ].
 proof.
-rewrite /XMSS_N => [#] n_val ??.
+rewrite /XMSS_N /XMSS_D /XMSS_TREE_HEIGHT /XMSS_FULL_HEIGHT => [#] n_val d_val h_val ??.
 proc => /=.
 seq 13 5 : (
   #pre /\
@@ -119,34 +119,210 @@ seq 13 5 : (
 
   idx_new{2} = idx{2} + W32.one
 ). 
-
     + inline {1} 13.
-      inline {1} 12.
       wp.
       ecall {1} (zero_addr_res addr{1}).
       auto => /> *.
-      split. 
-         * rewrite /zero_addr tP => i?.
-           rewrite get_setE // initiE //.
-         * admit.
-seq 1 0 : (#pre); first by admit.
-seq 2 0 : (#pre /\ to_uint t64{1} = to_uint mlen{1} + XMSS_SIG_BYTES). (* 2500 = XMSS_SIG_BYTES *) 
-    + auto => /> *; rewrite to_uintD of_uintK /#. 
-seq 1 0 : #pre; first by admit. (* memories are no longer equal *)
-seq 1 0 : (
-  #pre /\ 
-  to_uint idx{1} = to_uint (W32ofBytes (sub sk{1} 0 4)) /\
-  to_uint idx{1} = to_uint sk{2}.`Types.idx
+      admit.
+
+seq 1 0 : #pre.
+    + inline {1}; auto => /> *; by apply zero_addr_setZero.
+
+seq 0 1 : (
+  #{/~idx{2} = sk{2}.`Types.idx}
+   {/~sk{2} = _sk}
+   {/~0 <= to_uint sk{2}.`Types.idx < 2 ^ XMSS_FULL_HEIGHT - 1}pre /\ 
+  sk{2} = {| _sk with idx=idx_new{2} |} /\
+  0 < to_uint sk{2}.`Types.idx <= 2 ^ XMSS_FULL_HEIGHT 
 ).
-    + admit. (* Add lemma to Correctness Bytes *)
+    + auto => /> ?????H?. 
+      rewrite /XMSS_FULL_HEIGHT //= in H.
+      rewrite /XMSS_FULL_HEIGHT to_uintD.
+      do split => *; 1,3,4: by smt(@W32 pow2_32). 
+      simplify.
+      admit. (* Rever: Isto e falso *)
+
+
+
+seq 1 0 : (#pre).
+    + inline; wp; sp. 
+      while {1} (true) (to_uint bytes1{1} - to_uint i0{1}); auto => /> *; first by smt(@W64 pow2_64).
+      split; first by rewrite ultE /#.
+      rewrite ultE => ?. 
+      congr.
+      admit. (* This is false *)
+
+seq 2 0 : (#pre /\ to_uint t64{1} = to_uint mlen{1} + XMSS_SIG_BYTES).
+  + auto => /> *.
+    rewrite /XMSS_SIG_BYTES to_uintD_small of_uintK /#.
+
+seq 1 0 : (#pre).
+    + auto => /> &1 *.
+         admit.
+
+
+
+seq 1 1 : (#pre /\ to_list idx_bytes{1} = sub sk{1} 0 XMSS_INDEX_BYTES).
+    + auto => /> &1 &2 *.
+      apply (eq_from_nth witness); first by rewrite size_to_list size_sub /#.
+      rewrite size_to_list => i?.
+      rewrite get_to_list initiE // /DecodeSkNoOID get_of_list 1:/# nth_sub 1:/# get_of_list // /#.
+
+seq 1 0 : (#pre /\ to_uint idx{1} = to_uint sk{2}.`Types.idx /\ to_uint idx{1} < 2 ^ XMSS_FULL_HEIGHT - 1).
+
+    + admit.
+
+
+
+(* We dont enter this if statement because we assumed that the index is valid *)
 rcondf {1} 1.
-    + auto => /> &hr ???H H0 ?? H1. 
-      rewrite uleE of_uintK H1.  
+    + auto => /> &hr ???????????H.
       rewrite /XMSS_FULL_HEIGHT /= in H.
-      rewrite /(`<<`) ifT // /= /#. 
-rcondt {1} 1; first by auto => /> *; smt(@W8).
-seq 1 0 : (#pre); first by admit. (* fix this *)
-seq 4 0 : (#pre /\ sub sk{1} 0 4 = lenbytes_be32 idx_new{2} 4); first by admit.
+      rewrite uleE of_uintK /(`<<`) ifT // /#.
+
+(* We enter this if statement because we assumed that the index is valid *)
+rcondt {1} 1; first by auto => /> ; smt(@W8).
+
+seq 2 0 : (#pre /\ sub signature{1} 0 XMSS_INDEX_BYTES = to_list idx_bytes{1}).
+    + wp.
+      inline {1} 1.
+      inline {1} 5.
+      wp.
+      exists * idx_bytes{1}; elim * => P0.
+      ecall {1} (_memcpy_u8u8_3_3_post_p P0).
+      auto => /> &1 ????????? H *. 
+      rewrite H.
+      apply (eq_from_nth witness); first by rewrite /XMSS_INDEX_BYTES !size_sub.
+      rewrite size_sub // /XMSS_INDEX_BYTES => i?.
+      rewrite !nth_sub // /DecodeSkNoOID initiE 1:/# get_of_list 1:/# /= ifT //.
+      rewrite nth_cat ifT.
+           * rewrite !size_cat !valP n_val size_take // sizeW32toBytes ifT /#.
+      rewrite nth_cat ifT.
+           * rewrite !size_cat !valP n_val size_take // sizeW32toBytes ifT /#.
+      rewrite nth_cat ifT.
+           * rewrite !size_cat !valP n_val size_take // sizeW32toBytes ifT /#.
+      rewrite nth_cat ifT.
+           * rewrite size_take // sizeW32toBytes ifT /#.
+      rewrite nth_take // 1:/#.
+      rewrite -get_to_list H.
+      rewrite !nth_sub // /DecodeSkNoOID initiE 1:/# /=.
+      rewrite nth_cat ifT.
+           * rewrite !size_cat !valP n_val size_take // sizeW32toBytes ifT /#.
+      rewrite nth_cat ifT.
+           * rewrite !size_cat !valP n_val size_take // sizeW32toBytes ifT /#.
+      rewrite nth_cat ifT.
+           * rewrite !size_cat !valP n_val size_take // sizeW32toBytes ifT /#.
+      rewrite nth_cat ifT.
+           * rewrite size_take // sizeW32toBytes ifT /#.
+      rewrite nth_take // /#.
+
+seq 27 11 : (#{/~r{1} = W64.zero}post); last by auto => />.
+
+seq 2 0 : (#{/~to_uint t64{1} = to_uint mlen{1} + XMSS_SIG_BYTES}pre /\ 
+           t64{1} = idx{1} + W64.one); first by auto.
+
+seq 5 1 : (#pre /\ to_list buf{1} = val _R{2}).
+    + admit.
+
+seq 2 0 : (#pre /\ sub signature{1} XMSS_INDEX_BYTES n = val _R{2}).
+    + wp.
+      exists * buf{1}; elim * => P1.
+      call {1} (_x_memcpy_u8u8_post P1).
+      auto => /> &1 &2 ???????????H0 H1 ; split.
+           * apply (eq_from_nth witness); first by rewrite size_to_list size_sub.
+             rewrite size_sub // /XMSS_INDEX_BYTES => i?.             
+             rewrite nth_sub // initiE 1:/# /= ifF 1:/#.
+             rewrite (: idx_bytes{1}.[i] = nth witness (to_list idx_bytes{1}) i) 1:/# -H0 nth_sub //.
+           * apply (eq_from_nth witness); first by rewrite size_sub 1:/# valP.
+             rewrite size_sub 1:/# n_val => i?.
+             by rewrite nth_sub // initiE 1:/# /= ifT 1:/# -H1 /XMSS_INDEX_BYTES get_to_list.
+
+seq 1 0 : (#{/~t64{1} = idx{1} + W64.one}pre /\ to_list pub_root{1} = val root{2}).
+    + auto => /> &1 &2 *.
+      apply (eq_from_nth witness); first by rewrite size_to_list valP n_val.
+      rewrite size_to_list => i?.
+      rewrite get_to_list initiE //= /DecodeSkNoOID get_of_list 1:/# nth_cat ifT.
+          * rewrite !size_cat !valP n_val size_take //= sizeW32toBytes ifT /#.
+      rewrite nth_cat ifF.
+          * rewrite !size_cat !valP n_val size_take //= sizeW32toBytes ifT /#.
+      rewrite !size_cat !valP n_val size_take // sizeW32toBytes ifT /#.
+
+seq 3 2 : (#pre /\ val _M'{2} = to_list mhash{1}).
+    + wp.
+      admit.
+
+seq 2 0 : #pre; first by inline {1}; auto => /> &1 &2 *;rewrite !zero_addr_setZero //.
+
+seq 2 1 : (#pre /\ to_uint idx_tree{1} = to_uint idx_tree{2}).
+    + auto => /> &1 &2 *. 
+      rewrite  shr_div of_uintK //= h_val d_val /= /W32.
+      admit.
+
+seq 2 1 : (#pre /\ to_uint idx_leaf{1} = to_uint idx_leaf{2}).
+    + auto => /> &1 &2 *.
+      admit.
+
+seq 1 2 : (#{/~ots_addr{1} = zero_addr}
+            {/~address{2} = zero_addr}pre /\  
+           address{2} = ots_addr{1}).
+    + inline {1}; auto => /> &1 &2 *.
+      rewrite /set_tree_addr /set_layer_addr.
+      rewrite tP => i?.
+      rewrite get_setE //.
+      case (i = 2) => *.
+         * rewrite get_setE // ifT // #smt:(@W32 pow2_32).
+      rewrite get_setE //.
+      case (i = 1) => *.
+         * rewrite get_setE // ifF 1:/# get_setE // ifT //. 
+           rewrite (: 63 = 2^6 - 1) 1:/# and_mod // of_uintK.
+           rewrite /truncateu8 of_uintK //=.
+           rewrite /truncateu32 shr_div of_uintK /= /#. 
+      rewrite get_setE //.
+      case (i = 0) => *.
+         * by rewrite get_setE // ifF 1:/# get_setE // ifF 1:/# zero_addr_i.
+      by rewrite get_setE // ifF 1:/# get_setE // ifF 1:/#.
+
+seq 5 4 : (
+            to_uint _sm_ptr + XMSS_SIG_BYTES <= W64.max_uint /\
+            sm_ptr{1} = _sm_ptr /\ 
+            sk{1} = DecodeSkNoOID sk{2} /\ 
+            sig{2} = EncodeSignature (to_list signature{1})
+); last first.
+
+while {1}
+(#pre /\
+ 0 <= i{1} <= XMSS_SIG_BYTES /\
+ forall (k : int), 0 <= k < i{1} => loadW8 Glob.mem{1} (to_uint sm_ptr{1} + k) = signature{1}.[k])
+(XMSS_SIG_BYTES - i{1}); last first.
+  + auto => /> &1 *.
+    split => [/# | mem i].
+    split => [/# | ???].
+    have ->: i = XMSS_SIG_BYTES by smt().
+    rewrite /XMSS_SIG_BYTES => H.
+    congr.
+    apply (eq_from_nth witness); first by rewrite size_to_list /load_message size_mkseq of_uintK /=.
+    rewrite size_to_list => j?.
+    by rewrite /load_message get_to_list nth_mkseq //= -H.
+  + auto => /> &hr H?H0 H1?. 
+    rewrite /XMSS_SIG_BYTES in H0.
+    rewrite /XMSS_SIG_BYTES in H.
+    do split; 1,2,4: by smt().
+    move => k??.
+    rewrite /loadW8 /storeW8 get_setE. 
+    
+    case (k = i{hr}) => [-> | ?].
+      * rewrite ifT // to_uintD of_uintK #smt:(@W64 pow2_64).
+      * rewrite ifF; [by rewrite to_uintD of_uintK #smt:(@W64 pow2_64) |].
+        rewrite -H1 // /#.
+    
+
+admit.
+qed.
+
+
+
+(* ========================================================================================================================================= *)
+
 
 swap {2} 2 - 1.
 seq 1 1 : (
@@ -165,7 +341,7 @@ seq 0 1 : (#pre /\ sk{1} = DecodeSkNoOID sk{2}). (* Isto nao e #pre *)
 
 seq 1 0 : (#pre /\ to_list sk_prf{1} = val sk_prf{2}).
     + auto => /> &1 &2 *.
-      apply (eq_from_nth witness); first by rewrite valP n_val size_to_list.
+      apply (eq_from_nth witness); first by rewrite valP n_val _to_list.
       rewrite size_to_list => j?. 
       rewrite get_to_list initiE // => />.
       rewrite /DecodeSkNoOID get_of_list 1:/#.
